Weidenbach_Book/IsaSAT_Decide_LLVM.thy
@@ -2,6 +2,7 @@ theory IsaSAT_Decide_LLVM
   imports IsaSAT_Decide IsaSAT_VMTF_LLVM IsaSAT_Setup_LLVM
 begin
 
+(* Cannot find usage of this
 sepref_definition lit_of_found_atm_D_code
   is \<open>uncurry lit_of_found_atm_D\<close>
   :: \<open>[lit_of_found_atm_D_pre]\<^sub>a
@@ -14,22 +15,27 @@ sepref_definition lit_of_found_atm_D_code
   by sepref
 
 declare lit_of_found_atm_D_code.refine[sepref_fr_rules]
-
+*)
+(* Cannot find usage of this
 lemma lit_of_found_atm_hnr[sepref_fr_rules]:
   \<open>(uncurry lit_of_found_atm_D_code, uncurry lit_of_found_atm)
    \<in> [lit_of_found_atm_D_pre]\<^sub>a
-     phase_saver_conc\<^sup>k *\<^sub>a (option_assn uint32_nat_assn)\<^sup>d \<rightarrow>
+     phase_saver_assn\<^sup>k *\<^sub>a (option_assn uint32_nat_assn)\<^sup>d \<rightarrow>
      option_assn unat_lit_assn\<close>
   using lit_of_found_atm_D_code.refine[FCOMP lit_of_found_atm_D_lit_of_found_atm[unfolded convert_fref]] by simp
+*)
+(*sepref_register find_undefined_atm*)
 
-sepref_register find_undefined_atm
+(*
 sepref_definition find_unassigned_lit_wl_D_code
   is \<open>find_unassigned_lit_wl_D_heur\<close>
   :: \<open>isasat_unbounded_assn\<^sup>d \<rightarrow>\<^sub>a (isasat_unbounded_assn *a option_assn unat_lit_assn)\<close>
   supply [[goals_limit=1]]
   unfolding find_unassigned_lit_wl_D_heur_def isasat_unbounded_assn_def PR_CONST_def
   by sepref
+*)  
 
+(* will inline
 sepref_definition find_unassigned_lit_wl_D_fast_code
   is \<open>find_unassigned_lit_wl_D_heur\<close>
   :: \<open>isasat_bounded_assn\<^sup>d \<rightarrow>\<^sub>a (isasat_bounded_assn *a option_assn unat_lit_assn)\<close>
@@ -39,8 +45,9 @@ sepref_definition find_unassigned_lit_wl_D_fast_code
 
 declare find_unassigned_lit_wl_D_code.refine[sepref_fr_rules]
   find_unassigned_lit_wl_D_fast_code.refine[sepref_fr_rules]
+*)
 
-
+(*
 sepref_definition decide_lit_wl_code
   is \<open>uncurry decide_lit_wl_heur\<close>
   :: \<open>unat_lit_assn\<^sup>k *\<^sub>a isasat_unbounded_assn\<^sup>d \<rightarrow>\<^sub>a isasat_unbounded_assn\<close>
@@ -48,38 +55,176 @@ sepref_definition decide_lit_wl_code
   unfolding decide_lit_wl_heur_def isasat_unbounded_assn_def PR_CONST_def
     cons_trail_Decided_def[symmetric]
   by sepref
-
+*)
 
 sepref_definition decide_lit_wl_fast_code
   is \<open>uncurry decide_lit_wl_heur\<close>
   :: \<open>unat_lit_assn\<^sup>k *\<^sub>a isasat_bounded_assn\<^sup>d \<rightarrow>\<^sub>a isasat_bounded_assn\<close>
   supply [[goals_limit=1]]
-  unfolding decide_lit_wl_heur_def isasat_bounded_assn_def PR_CONST_def
-    cons_trail_Decided_def[symmetric]
+  unfolding decide_lit_wl_heur_def isasat_bounded_assn_def
   by sepref
 
-declare decide_lit_wl_code.refine[sepref_fr_rules]
-  decide_lit_wl_fast_code.refine[sepref_fr_rules]
+declare decide_lit_wl_fast_code.refine[sepref_fr_rules]
 
 
 sepref_register decide_wl_or_skip_D find_unassigned_lit_wl_D_heur decide_lit_wl_heur
-sepref_definition decide_wl_or_skip_D_code
-  is \<open>decide_wl_or_skip_D_heur\<close>
-  :: \<open>isasat_unbounded_assn\<^sup>d \<rightarrow>\<^sub>a bool_assn *a isasat_unbounded_assn\<close>
-  unfolding decide_wl_or_skip_D_heur_def PR_CONST_def
+
+find_theorems lit_of_found_atm
+
+find_theorems "\<langle>Id\<rangle>nres_rel = Id"
+
+lemma lit_of_found_atm_D_refine: "
+  \<lbrakk>lit_of_found_atm_D_pre (\<phi>, a); (\<phi>,\<phi>')\<in>Id; (a,a')\<in>Id\<rbrakk> \<Longrightarrow> lit_of_found_atm_D \<phi> a \<le>\<Down>Id (lit_of_found_atm \<phi>' a')"
+  using lit_of_found_atm_D_lit_of_found_atm unfolding convert_fref
+  by (auto dest!: frefD nres_relD)
+  
+thm decide_wl_or_skip_D_heur_def[unfolded find_unassigned_lit_wl_D_heur_def, no_vars]  
+  
+definition "decide_wl_or_skip_D_heur1 S \<equiv> doN {
+  (S, L) \<leftarrow> case S of (M, N, D, WS, Q, vm, \<phi>, clvls) \<Rightarrow> do {
+                          ((M, vm), L) \<leftarrow> isa_vmtf_find_next_undef_upd M vm;
+                          L \<leftarrow> lit_of_found_atm_D \<phi> L;
+                          RETURN ((M, N, D, WS, Q, vm, \<phi>, clvls), L)
+                        };
+  case L of None \<Rightarrow> RETURN (True, S) | Some L \<Rightarrow> do {
+                                           T \<leftarrow> decide_lit_wl_heur L S;
+                                           RETURN (False, T)
+                                         }
+  }"
+
+lemma decide_wl_or_skip_D_heur1_refine: "decide_wl_or_skip_D_heur1 S \<le> 
+  (decide_wl_or_skip_D_heur S)"
+  unfolding decide_wl_or_skip_D_heur1_def decide_wl_or_skip_D_heur_def find_unassigned_lit_wl_D_heur_def
+  (*using lit_of_found_atm_D_refine*)
+  apply (rule refine_IdD)
+  apply (refine_vcg lit_of_found_atm_D_refine)
+  apply (refine_dref_type)
+  by simp_all
+  
+  
+lemma bind_refine_same:
+  assumes "\<And>x. f x \<le> \<Down>R (g x)"
+  shows "doN { x \<leftarrow> m; f x} \<le>\<Down>R (doN { x \<leftarrow> m; g x})"  
+  using assms 
+  by (simp add: pw_le_iff refine_pw_simps; blast) 
+  
+term lit_of_found_atm_D  
+
+definition "lit_of_atm_D \<phi> L \<equiv> doN {
+  ASSERT (L<length \<phi>);
+  if \<phi>!L then RETURN (Pos L) else RETURN (Neg L)
+}"
+
+  
+lemma decide_wl_or_skip_D_heur2_refine: "doN {
+    let (M, N, D, WS, Q, vm, \<phi>, clvls) = S;
+    ((M, vm), L) \<leftarrow> isa_vmtf_find_next_undef_upd M vm;
+    if is_None L then let S = (M, N, D, WS, Q, vm, \<phi>, clvls) in RETURN (True, S)
+    else doN {
+      L \<leftarrow> lit_of_atm_D \<phi> (the L);
+      let S = (M, N, D, WS, Q, vm, \<phi>, clvls);
+      S \<leftarrow> decide_lit_wl_heur L S;
+      RETURN (False, S)
+    }
+  }
+  \<le>
+  decide_wl_or_skip_D_heur1 S"
+proof -
+  obtain M N D WS Q vm \<phi> clvls where SEQ: "S = (M, N, D, WS, Q, vm, \<phi>, clvls)" by (cases S)
+
+  show ?thesis
+    unfolding decide_wl_or_skip_D_heur1_def lit_of_atm_D_def lit_of_found_atm_D_def
+    apply (simp add: SEQ cong: if_cong)
+    apply (rule refine_IdD)
+    apply (rule bind_refine_same)
+    apply (simp split!: prod.splits; intro allI impI conjI; clarsimp)
+    done
+qed  
+  
+(* TODO: Move *)
+sepref_register isa_vmtf_find_next_undef  
+
+sepref_definition isa_vmtf_find_next_undef_code is 
+  "uncurry isa_vmtf_find_next_undef" :: "vmtf_remove_assn\<^sup>k *\<^sub>a trail_pol_fast_assn\<^sup>k \<rightarrow>\<^sub>a atom.option_assn"
+  unfolding isa_vmtf_find_next_undef_def vmtf_remove_assn_def
+  unfolding atom.fold_option
+  apply (rewrite in "WHILEIT _ \<hole>" short_circuit_conv)
   supply [[goals_limit = 1]]
-    find_unassigned_lit_wl_D_def[simp] image_image[simp]
+  apply annot_all_atm_idxs
   by sepref
+lemmas [sepref_fr_rules] = isa_vmtf_find_next_undef_code.refine  
+
+sepref_register update_next_search
+sepref_definition update_next_search_code is 
+  "uncurry (RETURN oo update_next_search)" :: "atom.option_assn\<^sup>k *\<^sub>a vmtf_remove_assn\<^sup>d \<rightarrow>\<^sub>a vmtf_remove_assn"
+  unfolding update_next_search_def vmtf_remove_assn_def
+  by sepref
+lemmas [sepref_fr_rules] = update_next_search_code.refine
+  
+sepref_register isa_vmtf_find_next_undef_upd  
+sepref_definition isa_vmtf_find_next_undef_upd_code is 
+  "uncurry isa_vmtf_find_next_undef_upd" 
+    :: "trail_pol_fast_assn\<^sup>d *\<^sub>a vmtf_remove_assn\<^sup>d \<rightarrow>\<^sub>a (trail_pol_fast_assn *a vmtf_remove_assn) *a atom.option_assn"
+  unfolding isa_vmtf_find_next_undef_upd_def
+  by sepref
+lemmas [sepref_fr_rules] = isa_vmtf_find_next_undef_upd_code.refine
+  
+find_consts name: lit name: assn
+
+find_theorems unat_lit_assn Neg
+
+sepref_register lit_of_atm_D
+sepref_definition lit_of_atm_D_code is "uncurry lit_of_atm_D" :: "(larray32_assn bool1_assn)\<^sup>k *\<^sub>a atom_assn\<^sup>k \<rightarrow>\<^sub>a unat_lit_assn"
+  unfolding lit_of_atm_D_def
+  apply annot_all_atm_idxs
+  by sepref_dbg_keep
+lemmas [sepref_fr_rules] = lit_of_atm_D_code.refine
+
+
+definition "make_isasat_bounded M N D WS Q vm \<phi> clvls = RETURN (M, N, D, WS, Q, vm, \<phi>, clvls)"
+
+lemma fold_make_isasat_bounded: "Let (M, N, D, WS, Q, vm, \<phi>, clvls) m = make_isasat_bounded M N D WS Q vm \<phi> clvls \<bind> m"
+  unfolding make_isasat_bounded_def by auto
+
+sepref_register make_isasat_bounded
+sepref_definition make_isasat_bounded_impl is "uncurry7 (make_isasat_bounded)"
+  :: "
+  trail_pol_fast_assn\<^sup>d *\<^sub>a arena_fast_assn\<^sup>d *\<^sub>a
+  conflict_option_rel_assn\<^sup>d *\<^sub>a
+  sint64_nat_assn\<^sup>d *\<^sub>a
+  watchlist_fast_assn\<^sup>d *\<^sub>a
+  vmtf_remove_assn\<^sup>d *\<^sub>a phase_saver_assn\<^sup>d *\<^sub>a (
+  uint32_nat_assn *a
+  cach_refinement_l_assn *a
+  lbd_assn *a
+  out_learned_assn *a
+  stats_assn *a
+  ema_assn *a
+  ema_assn *a
+  restart_info_assn *a
+  vdom_fast_assn *a
+  vdom_fast_assn *a
+  uint64_nat_assn *a
+  opts_assn *a arena_fast_assn)\<^sup>d  
+  \<rightarrow>\<^sub>a isasat_bounded_assn"
+  unfolding make_isasat_bounded_def isasat_bounded_assn_def
+  by sepref
+
+lemmas [sepref_fr_rules] = make_isasat_bounded_impl.refine  
+  
 
 sepref_definition decide_wl_or_skip_D_fast_code
   is \<open>decide_wl_or_skip_D_heur\<close>
-  :: \<open>isasat_bounded_assn\<^sup>d \<rightarrow>\<^sub>a bool_assn *a isasat_bounded_assn\<close>
-  unfolding decide_wl_or_skip_D_heur_def PR_CONST_def
+  :: \<open>isasat_bounded_assn\<^sup>d \<rightarrow>\<^sub>a bool1_assn *a isasat_bounded_assn\<close>
   supply [[goals_limit = 1]]
-    find_unassigned_lit_wl_D_def[simp] image_image[simp]
+  apply (rule hfref_refine_with_pre[OF decide_wl_or_skip_D_heur1_refine])
+  apply (rule hfref_refine_with_pre[OF decide_wl_or_skip_D_heur2_refine])
+  unfolding fold_make_isasat_bounded
+  unfolding atom.fold_option
+  apply (rewrite in "\<hole> \<rightarrow>\<^sub>a _" isasat_bounded_assn_def)
   by sepref
+  
 
-declare decide_wl_or_skip_D_code.refine[sepref_fr_rules]
-  decide_wl_or_skip_D_fast_code.refine[sepref_fr_rules]
+declare decide_wl_or_skip_D_fast_code.refine[sepref_fr_rules]
 
 end
